<?xml version="1.0" encoding="UTF-8"?>

<section xml:id="sect-applications-eigen">
  <title>Applications of Eigenvalues and Eigenvectors</title>

  <introduction>
    <p> We will develop a simple model of population growth in this section and show an example
      where eigenvalues and eigenvectors play an important role. </p>

    <p> Consider a population of a single species, perhaps a bacteria, which varies over time. Let <m>
      p_n</m> be the population at the <m>n</m>th time unit (day, month, year, \ldots). A simple
      model will be that the population at the next time will be proportional to the current
      population, thus <m>p_{n+1}
        = r p_n</m>. </p>

    <p> If the number of bacteria starting is 50, then <m>p_0=50</m> and the population doubles
      every time unit, so <m>r=2</m>, then</p>

    <p>
      <md>
        <mrow>p_1 \amp= 2 p_0 = 100 </mrow>
        <mrow>p_2 \amp = 2p_1 = 200 </mrow>
        <mrow>p_3 \amp = 2p_2 = 400</mrow>
      </md>
    </p>


    <p> and so on. In general </p>

    <p>
      <md>
        <mrow>p_1 \amp = r p_0 </mrow>
        <mrow>p_2 \amp = r p_1 = r^2 p_0 </mrow>
        <mrow>p_3 \amp = r p_2 = r^3 p_0 </mrow>
        <mrow>\vdots \amp = \vdots </mrow>
        <mrow>p_n \amp= r^n p_0</mrow>
      </md>
    </p>

    <p> From this model, the population increases without bound if <m>r \gt 1</m>, drops to zero if <m>r
      \lt 1</m> and if <m>r=1</m>, <m>p_n =p_0</m>.</p>

  </introduction>

  <subsection
    xml:id="sect-leslie-models">
    <title>Leslie Population Models</title>

    <p> The previous model actually works well for species like single-celled organisms, however,
      more advanced species will require a more complicated model. Consider a species, like some
      type of bird, that has two stages of life: juvenile and adult. We will also assume that the
      population of males and females are equal. The juvenile female cannot reproduce and the adult
      female can. Let <m>
        p_n</m> and <m>q_n</m> be the population of the juveniles and adults females at stage <m>n</m>.
      A simple model for growth is </p>

    <p>
      <md>
        <mrow>p_{n+1} \amp = k q_n </mrow>
        <mrow>q_{n+1} \amp = \alpha p_n + \beta q_n</mrow>
      </md>
    </p>

    <p>where at each stage the fraction <m>\alpha</m> of the juveniles survive to adulthood, and the
      population of the adults will produce a factor <m>k</m> juveniles. Finally, the fraction <m>
      \beta</m> of the adults survive one time unit. This linear system can be written as the matrix
      equation</p>

    <p>
      <me>
        \vec{p}_{n+1} = A \vec{p}_n
</me>
    </p>
    <p>where </p>

    <p>
      <md>
        <mrow>\vec{p} \amp=
          \begin{bmatrix}
          p \\ q
          \end{bmatrix}
          \amp A \amp =
          \begin{bmatrix}
          0 \amp k \\ \alpha \amp \beta
          \end{bmatrix}</mrow>
      </md>
    </p>

    <p>As a specific example, let's consider</p>

    <p>
      <me>
        A =
        \begin{bmatrix}
        0 \amp 2 \\
        0.3 \amp 0.5
        \end{bmatrix}
</me>
    </p>

    <p> The first line means that for every adult female, two juvenile females are produced. The
      second line means that 0.3 (30 percent) of the juveniles survive to adulthood and at each
      stage
      0.5 (50 percent) of the adults survive to the next stage. </p>

    <p> Let's see what happens to this population for some initial condition. Let's say that we have
      10 female adults and 0 juvenile adults. Then </p>

    <p>
      <me>
        \vec{p}_1 = A \vec{p}_0 =
        \begin{bmatrix}
        0 \amp 2 \\
        0.3 \amp 0.5
        \end{bmatrix}
        \begin{bmatrix}
        0\\ 10
        \end{bmatrix} =
        \begin{bmatrix}
        20 \\ 5
        \end{bmatrix}
</me>
    </p>


    <p> In general, </p>

    <p>
      <me>
        \vec{p}_n = A^n \vec{p}_0
</me>
    </p>

    <table>
      <title>
        Table of population values</title>
      <tabular>
        <row>
          <cell>year </cell>
          <cell>
            <m>p_n</m>
          </cell>
          <cell>
            <m>q_n</m>
          </cell>
          <cell>
            <m>T_n</m>
          </cell>
          <cell>
            <m>p_n/q_n</m>
          </cell>
          <cell>
            <m>T_{n+1}/T_n</m>
          </cell>
        </row>
        <row>
          <cell>0 </cell>
          <cell> 0 </cell>
          <cell> 10 </cell>
          <cell> 10 </cell>
          <cell> 0 </cell>
          <cell> </cell>
        </row>
        <row>
          <cell>1 </cell>
          <cell> 20 </cell>
          <cell> 5 </cell>
          <cell> 25 </cell>
          <cell> 4.00 </cell>
          <cell> 2.50 </cell>
        </row>
        <row>
          <cell>2 </cell>
          <cell> 10 </cell>
          <cell> 8 </cell>
          <cell> 18 </cell>
          <cell> 1.18 </cell>
          <cell> 0.74 </cell>
        </row>
        <row>
          <cell>3 </cell>
          <cell> 17 </cell>
          <cell> 7 </cell>
          <cell> 24 </cell>
          <cell> 2.34 </cell>
          <cell> 1.31 </cell>
        </row>
        <row>
          <cell>4 </cell>
          <cell> 14 </cell>
          <cell> 8 </cell>
          <cell> 22 </cell>
          <cell> 1.66 </cell>
          <cell> 0.96 </cell>
        </row>
        <row>
          <cell>5 </cell>
          <cell> 17 </cell>
          <cell> 8 </cell>
          <cell> 25 </cell>
          <cell> 2.00 </cell>
          <cell> 1.13 </cell>
        </row>
        <row>
          <cell>
            <m>\vdots</m>
          </cell>
        </row>
        <row>
          <cell>10 </cell>
          <cell> 22 </cell>
          <cell> 12 </cell>
          <cell> 34 </cell>
          <cell> 1.87 </cell>
          <cell> 1.06 </cell>
        </row>
        <row>
          <cell>11 </cell>
          <cell> 24 </cell>
          <cell> 12 </cell>
          <cell> 36 </cell>
          <cell> 1.88 </cell>
          <cell> 1.07 </cell>
        </row>
        <row>
          <cell>12 </cell>
          <cell> 25 </cell>
          <cell> 13 </cell>
          <cell> 38 </cell>
          <cell> 1.88 </cell>
          <cell> 1.06</cell>
        </row>
      </tabular>
    </table>


    <p>We'd like to explain what is going on here. As we will show, the eigenvalues are important.
      The characteristic equation is </p>

    <p>
      <me>
        \lambda^2 -0.5 \lambda -0.6 = 0
</me>
    </p>
    <p>which has the solutions </p>

    <p>
      <me>
        \lambda = \frac{0.5 \pm \sqrt{0.25 + 2.4}}{2} \approx 1.06, -0.56
</me>
    </p>

    <p>The eigenvectors are </p>

    <p>
      <md>
        <mrow>\vec{v}_1 \amp =
          \begin{bmatrix}
          1.88 \\ 1
          \end{bmatrix} \amp \vec{v}_2 \amp =
          \begin{bmatrix}
          -3.54 \\1
          \end{bmatrix}</mrow>
      </md>
    </p>

    <p> Assume that <m>\lambda_1</m> and <m>\lambda_2</m> are the eigenvalues of <m>A</m> and <m>
      \vec{v}_1</m> and <m>\vec{v}_2</m> are the eigenvectors. If <m>\vec{v}_1</m> and <m>\vec{v}_2</m>
      are linearly independent, then we can write </p>

    <p>
      <me>
        \vec{p}_0 = a_1 \vec{v}_1 + a_2 \vec{v}_2
</me>
    </p>

    <p>for some real numbers <m>a_1</m> and <m>a_2</m>. Let's use the matrix equations above to find <m>
      \vec{p}_1</m>,</p>

    <p>
      <md>
        <mrow>\vec{p}_1 \amp = A \vec{p}_0 = A (a_1 \vec{v}_1 + a_2 \vec{v}_2) </mrow>
        <mrow>\amp = a_1 A \vec{v}_1 + a_2 A \vec{v}_2 </mrow>
        <mrow>\amp = a_1 \lambda_1 \vec{v}_1 + a_2 \lambda_2 \vec{v}_2</mrow>
      </md>
    </p>

    <p>similarly, </p>

    <p>
      <md>
        <mrow>\vec{p}_2 \amp = A \vec{p}_1 = A(a_1 \lambda_1 \vec{v}_1 + a_2 \lambda_2 \vec{v}_2)</mrow>
        <mrow>\amp= a_1 \lambda_1 A \vec{v}_1 + a_2 \lambda_2 A \vec{v}_2 </mrow>
        <mrow>\amp = a_1 \lambda_1^2 \vec{v}_1 + a_2 \lambda_2^2 \vec{v}_2</mrow>
      </md>
    </p>

    <p> Now assume that <m>|\lambda_1|>|\lambda_2|</m> and factor <m>\lambda_1^n</m> out from the
      equation above: </p>

    <p>
      <me>
        \vec{p}_n = \lambda_1^n \biggl( a_1 \vec{v}_1 + a_2 \frac{\lambda_2^n}{\lambda_1^n}
        \vec{v}_2 \biggr)
</me>
    </p>

    <p>as <m>n</m> increases the ratio <m>(\lambda_2/\lambda_1)^n</m> goes to zero, so </p>

    <p>
      <me>
        \vec{p}_n \approx a_1 \lambda_1^n \vec{v}_1
</me>
    </p>

  </subsection>

  <subsection xml:id="sect-second-order-de">
    <title>Second-Order Differential Equations Systems</title>

    <p> Consider a mass-spring system: </p>

    <figure>
      <caption>
        Find a point on a line that minimizes distance
      </caption>
      <image width="50%">
        <latex-image>
          <![CDATA[
      \begin{tikzpicture} \draw (0,2) -- (0,0) -- (7,0);
      \draw[decorate,decoration={coil,segment length=4pt}] (0,0.5) -- (2.5,0.5)
        node [midway,above] {$k_1$};
      \draw (2.5,0) rectangle (3.5,1);
      \draw (3,0.5) node {$x_1$};
      \draw[decorate,decoration={coil,segment length=4pt}] (3.5,0.5) -- (5.5,0.5)
        node [midway,above] {$k_2$};
      \draw (5.5,0) rectangle (6.5,1);
      \draw (6,0.5) node {$x_2$};
      \end{tikzpicture}
      ]]>
    </latex-image>
      </image>
    </figure>

    <p>where <m>x_1</m> and <m>x_2</m> are the positions of the masses <m>m_1</m> and <m>m_2</m>
      relative to the unstretched spring positions and <m>k_1</m> and <m>k_2</m> are the spring
      constants of the two springs. The mass spring system above can be modeled using the 2nd order
      system of differential equations. </p>

    <p>
      <md>
        <mrow>m_1 x_1 '' \amp = - k_1 x_1 + k_2 (x_2-x_1) </mrow>
        <mrow>m_2 x_2 '' \amp = - k_2 (x_2-x_1) .</mrow>
      </md>
    </p>

    <p>This can be written in matrix form as </p>

    <p>
      <me>
        M \vec{x}'' = K\vec{x}
</me>
    </p>
    <p>with</p>


    <p>
      <md>
        <mrow>M \amp = \begin{bmatrix}
          m_1 \amp 0 \\ 0 \amp m_2
          \end{bmatrix}
          \amp
          K \amp =\begin{bmatrix}
          -(k_1+k_2) \amp k_2 \\ -k_2 \amp k_1
          \end{bmatrix}</mrow>
      </md>
    </p>

    <p> where <m>M</m> is the mass matrix and <m>K</m> is called the stiffness matrix, which can
      take other forms depending on the connectedness of the spring system. Since <m>M</m> is
      nonsingular, we can find <m>M^{-1}</m> and write the system above as: </p>

    <p>
      <me>
        \vec{x}'' = A \vec{x}
</me>
    </p>

    <p> where <m>A = M^{-1} K</m>. </p>
  </subsection>

  <subsection xml:id="sect-solutions-of-second-order-de">
    <title>Solutions of <m>\vec{x}''= A\vec{x}</m>
    </title>

    <p> Let <m>v</m> be an eigenvector of <m>A</m>, with eigenvalue <m>\lambda = \alpha^2</m>, then <m>\vec{x}
      =\vec{v}(c_1e^{\alpha t} + c_2 e^{-\alpha t})</m> is a solution. </p>

    <p>
      <md>
        <mrow>\vec{x}'' \amp = \alpha^2 \vec{v} (c_1 e^{\alpha t}+ c_2 e^{-\alpha t}) </mrow>
        <mrow>\amp = A \vec{v}(c_1e^{\alpha t} + c_2 e^{-\alpha t})</mrow>
      </md>
    </p>

    <p> if <m>\lambda \lt 0</m>, then the <m>\lambda = - \omega^2</m> and the solution is: </p>

    <p>
      <me>
        \vec{x} = \vec{v} (a \cos \omega t + b \sin \omega t)
</me>
    </p>

    <p>If <m>\lambda = 0</m> is an eigenvalue of <m>A</m> with corresponding eigenvector <m>
      \vec{v}_0</m>, then the part of the solution associate with this is: </p>

    <p>
      <me>
        \vec{x}(t) = (a_0 + b_0 t) \vec{v}_0
</me>
    </p>


    <theorem>
      <statement>
        <p> If the <m>n \times n</m> matrix <m>A</m> has distinct negative eigenvalues <m>-\omega_1^2,
          -\omega_2^2, \ldots, -\omega_n^2</m> with associated real eigenvectors, then a general
          solution to </p>

        <p>
          <me>
            \vec{x''} = A x
          </me>
        </p>

        <p>is given by</p>

        <p>
          <me>
            \vec{x} = \sum_{i=1}^n (a_i \cos \omega_i t + b_i \sin \omega_i t)\vec{v}_i
          </me>
        </p>
        <p> where <m>a_i</m> and <m>b_i</m> arbitrary constants. If <m>\lambda = 0</m> is an
          eigenvalue of <m>A</m> with corresponding eigenvector <m>\vec{v}_0</m>, then the part of
          the solution associate with this is: </p>

        <p>
          <me>
            \vec{x}(t) = (a_0 + b_0 t) \vec{v}_0
</me>
        </p>
      </statement>

    </theorem>

    <example>
      <statement>
        <p> Consider the mass-spring system above with <m>m_1=1</m>, <m>m_2=2</m>, <m>k_1 = 1</m>,
          and <m>k_2
            = 2</m>, then the mass matrix and stiffness matrix are: </p>

        <p>
          <md>
            <mrow>M \amp =
              \begin{bmatrix}
              1 \amp 0 \\ 0 \amp 2
              \end{bmatrix} \amp
              K \amp = \begin{bmatrix}
              -3 \amp 2 \\ -2 \amp 4 \end{bmatrix}</mrow>
          </md>
        </p>

        <p> resulting in the system: </p>

        <p>
          <me>
            \vec{x}'' = \begin{bmatrix}
            -3 \amp 2 \\ -1 \amp 2
            \end{bmatrix} \vec{x}
</me>
        </p>

        <p> The
          eigenvalues and eigenvectors are: </p>

        <p>
          <md>
            <mrow> \lambda_1 \amp = -4 \amp \vec{v}_1 \amp = (-2,1)^T </mrow>
            <mrow>\lambda_2 \amp = -1 \amp \vec{v}_2 \amp = (1,1)^T</mrow>
          </md>
        </p>

        <p>
          Therefore the solution is:
</p>

        <p>
          <men xml:id="eq-mass-spring-solution">
            \vec{x} = (a_1 \cos 2t + b_1 \sin 2t) \begin{bmatrix}
            -2 \\ 1
            \end{bmatrix} + (a_2 \cos t + b_2 \sin t) \begin{bmatrix}
            1 \\1
            \end{bmatrix}
          </men>
        </p>

        <p> Next, let's find the values of the <m>a</m>'s and <m>b</m>'s if <m>x_1=1</m> and <m>
          x_2=2</m> when <m>
            t=0</m> or </p>

        <p>
          <me>
            \vec{x}(0) = \begin{bmatrix}
            1 \\ 2
            \end{bmatrix}
</me>
        </p>

        <p>and <m>\vec{x}'(0)=\vec{0}</m>. First use the initial value <m>\vec{x}(0)</m> in (<xref
            ref="eq-mass-spring-solution" />), </p>

        <p>
          <me>
            \begin{bmatrix}
            1 \\ 2
            \end{bmatrix} = a_1 \begin{bmatrix}
            -2 \\ 1
            \end{bmatrix} + a_2 \begin{bmatrix}
            1 \\ 1
            \end{bmatrix}
</me>
        </p>

        <p> and this is true when <m>a_1=1/3</m> and <m>a_2=5/3</m>. To find <m>b_1</m> and <m>b_2</m>,
          differentiate (<xref ref="eq-mass-spring-solution" />), </p>


        <p>
          <md>
            <mrow>\vec{x}'(t) \amp = (-2a_1 \sin 2t + 2b_1
              \cos 2t ) \begin{bmatrix} -2 \\ 1 \end{bmatrix} + (-a_2 \sin t + b_2 \cos t)
              \begin{bmatrix} 1
              1 \end{bmatrix} </mrow>
          </md>
        </p>
        <p>and evaluate it at <m>t=0</m>
        </p>

        <p>
          <me>
            \vec{x}'(0) = \begin{bmatrix} 0 \\ 0
            \end{bmatrix} = 2b_1 \begin{bmatrix} -2 \\ 1 \end{bmatrix} + 2b_2 \begin{bmatrix} 1 \\ 1
            \end{bmatrix}
</me>
        </p>

        <p>or <m>b_1=0</m> and <m>b_2=0</m>. The solution with the given initial condition, </p>

        <p>
          <me>
            \vec{x}(t) = \frac{1}{3} \cos 2t \begin{bmatrix}
            -2 \\ 1
            \end{bmatrix} + \frac{5}{3} \cos t \begin{bmatrix}
            1 \\ 1
            \end{bmatrix}
</me>
        </p>

        <p> The value of <m>x_1</m> and <m>x_2</m>, the position of the two masses are the first and
          second components. A plot of these two are: </p>


        <figure>
          <caption>
            Solution of a second-order differential equation.
          </caption>
          <image width="90%" xml:id="plot-second-order-de-solution">
            <latex-image>
      <![CDATA[
\begin{tikzpicture}[xscale=0.5,yscale=1.5]
\draw[->] (-10,0) -- (10,0) node [above right] {$x$};
\draw[->] (0,-2.25) -- (0,2.25) node [above right] {$y$};

% this draws all the fractional multiples of pi

%\foreach \x/\num/\den/\neg in
% {0.5*pi/\pi/2/,1.5*pi/3\pi/2/,-0.5*pi/\pi/2/-,-1.5*pi/3\pi/2/-}
%  \draw ({\x},0.1) -- ({\x},-0.1) node [below] {$\neg \frac{\num}{\den}$};

% this draws all non fractional multiples of pi

\foreach \x/\val in {pi/\pi,2*pi/2\pi,3*pi/3\pi,-pi/-\pi,-2*pi/-2\pi,-3*pi/-3\pi}
    \draw (\x,0.1) -- (\x,-0.1) node [below] {$\val$};

\foreach \y in {-2,-1,1,2} \draw (0.1,\y) -- (-0.1,\y) node [left] {$\y$};


\draw plot[domain=-10:10,samples=100] (\x,{-2/3*cos(2*\x r)+5/3*cos(\x r)});
\draw[dashed] plot[domain=-10:10,samples=100] (\x,{1/3*cos(2*\x r)+5/3*cos(\x r)});

\end{tikzpicture}
]]>
</latex-image>
          </image>
        </figure>

      </statement>
    </example>
  </subsection>
</section>