<?xml version="1.0" encoding="UTF-8" ?>
<section xml:id="sec-bessel-eqn">
	<title>Bessel's equation and Bessel Functions</title>
	<introduction>
		<p>
			Bessel's equation is
		</p>

		<p>
			<men xml:id="eq-bessel-eqn">
				x^2 y'' + x y' + (x^2-\nu^2)y = 0
			</men>
		</p>

		<p>
			A solution can be obtained by a <em>power series solution</em> and represented as
		</p>

		<p>
			<me>
				J_{\nu} (x) = \frac{x^{\nu}}{2^{\nu}} \sum_{m=0}^{\infty} \frac{(-1)^m}{2^m m! \Gamma(m+\nu+1)} x^{2m}
			</me>
		</p>

		<p>
			where <m>\Gamma</m> is the gamma function, a generalized factorial.
			The function <m>J_{\nu}(x)</m> is called the <term>Bessel Function of the first kind</term>.
			We are often interested in solutions of <xref ref="eq-bessel-eqn" /> in which <m>\nu=n</m> is an integer.
			If this is the case, then <m>J_n(x)</m> and <m>J_{-n}(x)</m> are two linearly independent solutions.
			The power series representation in this case is
		</p>

		<p>
			<men xml:id="eq-bessel-function-power-series">
				J_{n} (x) = \frac{x^{n}}{2^{n}} \sum_{m=0}^{\infty} \frac{(-1)^m}{2^m m! (m+n)!} x^{2m}
			</men>
		</p>
	</introduction>

	<subsection>
		<title>Propeties of <m>J_n(x)</m></title>
		<p>
			The following is a plot of <m>J_0(x)</m> (solid line) and <m>J_1(x)</m> (dashed line) on
			<m>0 \leq x \leq 10</m>.
			Each of the Bessel functions have osciallatory behavior with decay and an infinite
			number of roots for <m>x \geq 0</m>.
			Also note that the roots of <m>J_1</m> are between the roots of <m>J_0</m>.
		</p>

		<figure xml:id="fig-bessel">
			<caption> A plot of the bessel functions <m>J_0</m> and <m>J_1</m> on <m>[0,10]</m>.</caption>
			<image width="75%" xml:id="plot-bessel">
				<latex-image>
				<![CDATA[
				\begin{tikzpicture}[yscale=3]
				\draw[->] (-0.5,0) -- (10.5,0) node [above right] {$x$};
				\foreach \x in {1,2,...,10} \draw (\x,0.05) -- (\x, -0.05) node [below] {\x};
				\foreach \y in {-1,1} \draw (0.1,\y) -- (-0.1,\y) node [left] {\y};
				\draw[->] (0,-1.1) -- (0,1.1) node [above right] {$y$};
				\draw plot[domain=0:4,samples=75] (\x,{(.1070175340+(-.3197655443+(.1317665405+(0.03420779066-0.009123904620*\x)*(\x-2))*(\x-2))*(\x-2))/(.4782168796+(-.1963783133+(0.03225662346-0.009674608375*\x)*(\x-2))*(\x-2))});
				\draw plot[domain=4:8,samples=75] (\x, {(0.38882689e-1+(0.67993679e-1+(-0.304195383e-1+(-0.1854623075e-1+0.2117043641e-2*\x)*(\x-6))*(\x-6))*(\x-6))/(.2580479835+(-0.225929762e-1+(0.1684428220e-1-0.1419604109e-2*\x)*(\x-6))*(\x-6))});
				\draw plot[domain=8:10,samples=75] (\x, {(-0.7016077e-2+(-0.17665130e-1+(0.81186790e-2+(0.7847342517e-2-0.6999609674e-3*\x)*(\x-9))*(\x-9))*(\x-9))/(0.77668449e-1+(-0.153635550e-1+(0.9679747603e-2-0.8086687126e-3*\x)*(\x-9))*(\x-9))});
				\draw[dashed] plot[domain=0:5,samples=100] (\x, {(.6293300006+(-.2276493766+(-.2208737473+(-0.1166308301e-1+0.1029876752e-1*\x)*(\x-2.5))*(\x-2.5))*(\x-2.5))/(1.265426981+(.1713608410+(0.2607601937e-1+0.8783305461e-2*\x)*(\x-2.5))*(\x-2.5))});
				\draw[dashed] plot[domain=5:10,samples=100] (\x,{(0.18515418e-1+(0.31837218e-1+(-0.145966941e-1+(-0.9991569388e-2+0.9863389544e-3*\x)*(\x-7.5))*(\x-7.5))*(\x-7.5))/(.136655698+(-0.154778221e-1+(0.1328463355e-1-0.1109859561e-2*\x)*(\x-7.5))*(\x-7.5))});
				\end{tikzpicture}
				]]>
				</latex-image>
			</image>
		</figure>

		<p>
			Using <xref ref="eq-bessel-function-power-series" />, it can be shown that
		</p>

		<p>
			<me>
				J_n(0) = \begin{cases}
				1 \amp \text{if $n=0$} \\
				0 \amp \text{otherwise}
				\end{cases}
			</me>
		</p>

		<p>
			In addition, using the power series representation, one can show that the other solution of <xref ref="eq-bessel-eqn" /> can be written:
		</p>

		<p>
			<me>
				J_{-n}(x) = (-1)^n J_n(x)
			</me>
		</p>

		<p>
			However for <m>n &lt; 0</m>,<m>J_n(x)</m> has a term <m>x^{-n}</m> which means that it is
			undefined at <m>x=0</m>, which is generally why it not relevant as we will show later.
			There are a number of identities that are useful for understanding Bessel functions.
			Two of these are shown in the follow lemma.
		</p>

		<lemma xml:id="lem-bessel-identities">
			<statement>
				<p>
					Consider <m>n\geq 1</m>, where <m>n</m> is an integer.
					Then
				</p>

				<p>
					<md>
						<mrow number="yes" xml:id="eq-bessel-id1">\frac{d}{dx} \bigl( x^n J_n(x) \bigr) \amp = x^n J_{n-1} (x) </mrow>
						<mrow number="yes" xml:id="eq-bessel-id2">\frac{d}{dx} \bigl( x^{-n} J_n(x) \bigr) \amp = -x^{-n} J_{n+1} (x)</mrow>
					</md>
				</p>

				<p>
					for all <m>x &gt; 0</m>.
				</p>
			</statement>


			<proof>
				<p>
					First we will prove <xref ref="eq-bessel-id1" />.
					Using <xref ref="eq-bessel-function-power-series" />, we can write
				</p>

				<p>
					<md>
						<mrow>x^nJ_n(x) \amp = x^n \biggl( \frac{x^{n}}{2^{n}} \sum_{m=0}^{\infty} \frac{(-1)^m}{2^m m! (m+n)!} x^{2m} \biggr) </mrow>
						<mrow>\amp = \sum_{m=0}^{\infty} \frac{(-1)^m}{2^{m+n} m! (m+n)!} x^{2m+2n} </mrow>
					</md>
				</p>

				<p>
					and differentiating,
				</p>

				<p>
					<md>
						<mrow>\frac{d}{dx} \bigl(x^nJ_n(x)\bigr) \amp =  \sum_{m=0}^{\infty} \frac{(-1)^m(2m+2n)}{2^{m+n} m! (m+n)!} x^{2m+2n-1} </mrow>
						<mrow>\amp = \frac{x^{n-1}}{2^{n-1}}  \sum_{m=0}^{\infty} \frac{(-1)^m2(m+n)}{2^{m+1} m! (m+n)!} x^{2m+n} </mrow>
						<mrow>\amp = x^n \biggl(\frac{x^{n-1}}{2^{n-1}}  \sum_{m=0}^{\infty} \frac{(-1)^m}{2^{m} m! (m+n-1)!} x^{2m}) </mrow>
						<mrow>\amp  = x^{n} J_{n-1}(x) </mrow>
					</md>
				</p>

				<p>
					The proof for <xref ref="eq-bessel-id2" /> is very similar and is not shown.
				</p>
			</proof>
		</lemma>

		<p>
			In addition, there are another two identities for Bessel functions that are often called recurrence relationships.
		</p>

		<lemma xml:id="lem-bessel-recurrence">
			<statement>
				<p>
					Let <m>n\geq 1</m> for <m>n</m> an integer and <m>x &gt; 0</m>, then
				</p>

				<p>
					<md>
						<mrow number="yes" xml:id="eq-bessel-recur1">x(J_{n-1}+J_{n+1}) \amp = 2n J_n</mrow>
						<mrow number="yes" xml:id="eq-bessel-recur2"> J_{n-1} - J_{n+1} \amp = 2 J'_n </mrow>
					</md>
				</p>
			</statement>


			<proof>
				<p>
					If we use the product rule to expand <xref ref="eq-bessel-id1" /> and <xref ref="eq-bessel-id2" />, we get
				</p>

				<p>
					<md>
						<mrow>n x^{n-1} J_n(x) + x^n J'_n(x) \amp = x^n J_{n-1} (x)  </mrow>
						<mrow>-nx^{-n-1} J_n(x) +x^{-n} J'_n(x) \amp = - x^{-n} J_{n+1}(x) </mrow>
					</md>
				</p>

				<p>
					and multiply the first equation by <m>x^{1-n}</m> and the second by <m>x^{1+n}</m>, one gets
				</p>

				<p>
					<md>
						<mrow>n J_n + x J'_n \amp = xJ_{n-1} </mrow>
						<mrow>-nJ_n+xJ'_n \amp = -xJ_{n+1}</mrow>
					</md>
				</p>

				<p>
					Adding the two above equations and dividing through by <m>x</m> results in <xref ref="eq-bessel-recur1" />
					whereas subtracting the bottom equation from the top results in <xref ref="eq-bessel-recur2" />.
				</p>
			</proof>
		</lemma>

		<p>
			These properties can now be used to find higher order Bessel functions, the derivatives of Bessel
			functions as well as the closed form of some integrals as shown in the next three examples.
		</p>

		<example xml:id="ex-bessel-J3">
			<statement>
				<p>
					Use the identities in <xref ref="lem-bessel-identities" /> and <xref ref="eq-bessel-recur1" />
					to find <m>J_3</m> in terms of <m>J_0</m> and <m>J_1</m>.
				</p>
			</statement>

			<solution>
				<p>
					Let <m>n=2</m> in <xref ref="eq-bessel-recur1" /> or
				</p>

				<p>
					<md>
						<mrow>x (J_1 + J_3) \amp = 4J_2 \amp\amp\text{solving for $J_3$} </mrow>
						<mrow>J_3 \amp = \frac{4}{x} J_2 - J_1 </mrow>
					</md>
				</p>

				<p>
					use <xref ref="eq-bessel-recur1" /> again with <m>n=1</m>
					or <m>x(J_0 + J_2) = 2J_1</m> which can be written <m>J_2 = (2/x)J_1 -J_0</m>
				</p>

				<p>
					<md>
						<mrow>\amp = \frac{4}{x} \biggl( \frac{2}{x} J_1 - J_0 \biggr) - J_1 </mrow>
						<mrow>J_3 \amp = \biggl( \frac{8}{x^2} -1\biggr) J_1 - \frac{2}{x} J_0 </mrow>
					</md>
				</p>
			</solution>
		</example>

		<p>
			The above technique can be used to find <m>J_n</m> where <m>n</m> is an integer in terms
			of <m>J_0</m> and <m>J_1</m>, showing the importance of the first two Bessel functions.
			The next example shows how to calculate the derivatives of the first two Bessel functions.
		</p>

		<example>
			<statement>
				<p>
					Use the identities in lemmas <xref ref="lem-bessel-identities" /> and <xref ref="lem-bessel-recurrence" /> to
					find <m>J'_0</m> and <m>J'_1</m> in terms of <m>J_0</m> and <m>J_1</m>.
				</p>
			</statement>

			<solution>
				<p>
					First, differentiate <xref ref="eq-bessel-recur1" /> with <m>n=1</m> to get
				</p>

				<p>
					<md>
						<mrow>x (J'_0 +J'_2) + J_0 + J_2 \amp = 2 J' _1  \quad\text{solving for $xJ'_0$} </mrow>
						<mrow>xJ'_0 \amp = 2J'_1 -J_0 - J_2 - xJ'_2 </mrow>
					</md>
				</p>

				<p>
					using <xref ref="eq-bessel-recur2" /> with <m>n=1</m> and <m>n=2</m>,
				</p>

				<p>
					<md>
						<mrow>xJ'_0 \amp = (J_0 - J_2) -J_0 -J_2 - \frac{xJ_1 - xJ_3}{2} </mrow>
						<mrow>\amp  = -2J_2 -\frac{xJ_1 - xJ_3}{2} </mrow>
					</md>
				</p>

				<p>
					Using <xref ref="eq-bessel-recur1" /> with <m>n=1</m>
				</p>

				<p>
					<md>
						<mrow>\amp = \frac{-x(J_1+J_3)}{2} - x\frac{J_1 -J_3}{2} = -xJ_1 </mrow>
					</md>
				</p>

				<p>
					and finally dividing through by <m>x</m>
				</p>

				<p>
					<me>
						J'_0  = -J_1
					</me>
				</p>
			</solution>
		</example>

		<example>
			<statement>
				<p>
					Evaluate <m>\int x^4 J_1 (x) \, dx</m>.
				</p>
			</statement>

			<solution>
				<p>
					Integrating this by parts with <m>u=x^2</m> and <m>du = x^2 J_1\, dx</m> results in
				</p>

				<p>
					<me>
						\int x^4 J_1 \, dx = \int x^2 (x^2 J_1) \,dx = x^2 (x^2 J_2) - \int x^2 J_2 (2x) \,dx - 2 \int x^3 J_2 \, dx
					</me>
				</p>

				<p>
					where <m>(x^2 J_2)'=x^2 J_1</m> is used from <xref ref="eq-bessel-id1" />.
					Next, if we again apply <xref ref="eq-bessel-id1" /> with <m>n=3</m>, to the last integral, we get
				</p>

				<p>
					<me>
						\int x^4 J_1 \, dx = x^4 J_2 -2x^3 J_3 + C
					</me>
				</p>
			</solution>
		</example>
	</subsection>

	<subsection>
		<title>Roots of the Bessel functions</title>
		<p>
			There is not an analytic way to find the roots of any of the bessel functions,
			so we will resort to numerical approximation.
			Many Computer Algebra Systems and
			scientific computing languages have bessel functions built in and roots can be
			found with techniques such as Newton's method or bisection.
		</p>

		<p>
			In general, the <m>i</m>th root of <m>J_0(x)</m> is between <m>(i-1)\pi</m> and
			<m>i\pi</m>, so the following Maple code will find the first 50.
		</p>

		<p>
			<me>
				\sigma := \text{[seq(fsolve(BesselJ(0,x)=0,x,(i-1)\cdot\pi,i\cdot\pi))]}
			</me>
		</p>

		<p>
			The first ten values are:  <m>\{2.404825558, 5.520078110, 8.653727913, 11.79153444, \\14.93091771, 18.07106397, 21.21163663, 24.35247153, 27.49347913, 30.63460647\}</m>.
		</p>
	</subsection>
</section>