<?xml version="1.0" encoding="UTF-8"?>
<section xml:id="sect-linear-ode">
	<title>Linear ordinary differential equations</title>
	<introduction>
		<p>
			As discussed in section <xref ref="sect-part-deriv-diff-eqns" />, a differential equation is ordinary if
			the derivatives are ordinary.
			Additionally, it is linear if it is linear in its dependent
			variable and derivatives of the dependent variable.
			We investigate the solution of some classes of
			linear ordinary differential equations in this section.
			Let's assume that <m>y</m> is the dependent variable and <m>x</m> is the independent variable.
			The most general <m>n</m>th order ordinary linear differential equation as the form:
		</p>

		<p>
			<men xml:id="eq-ODE-linear">
				a_n(x) y^{(n)} + a_{n-1}(x) y^{(n-1)} + \cdots + a_1(x) y' + a_0 (x) y = f(x)
			</men>
		</p>

		<p>
			In the most general terms, this differential equation is very difficult to solve despite being linear.
			However, there are cases when this has nice solutions.
			For the most part, we'll look at such equations in this section.
		</p>
	</introduction>

	<subsection>
		<title>Second-order Constant-Coefficient Homogeneous differential equations
		</title>

		<p>
			The most important ordinary differential equations that arise from solving the wave and heat
			equation are 2nd-order constant coefficient homogeneous differential equations.
			If <m>f(x) \equiv 0</m> in <xref ref="eq-ODE-linear" />, then it is called homogeneous and if the
			coefficients of the <m>y</m> terms and its derivatives are not dependent on <m>x</m>, then the equation is constant-coefficient.
			A general 2nd-order ODE with these characteristics can be written:
		</p>

		<p>
			<me>
				a y'' + b y' + cy = 0
			</me>
		</p>

		<p>
			where <m>a,b,c</m> are real constants.
			To solve these, if we let <m>y=e^{rx}</m> and substitute this into the ODE,
		</p>

		<p>
			<md>
				<mrow>ar^2 e^{rx} + br e^{rx} + ce^{rx} \amp = 0 </mrow>
				<mrow>e^{rx}(ar^2 + br +c) \amp = 0 </mrow>
			</md>
			and since <m>e^{rx}</m> is never 0
			<md>
				<mrow>ar^2+br+c=0</mrow>
			</md>
		</p>

		<p>
			is called the <term>characteristic equation</term> related to the ODE.
			In general, there are two solutions to this equation, <m>r_1</m> and <m>r_2</m>.
			The general solution to the equation will thus be
		</p>

		<p>
			<me>
				y = c_1 e^{r_1 x} + c_2 e^{r_2 x}
			</me>
		</p>

		<example xml:id="ex-solution-DE-image">
			<statement>
				<p>
					Find the general solution to
				</p>

				<p>
					<me>
						y'' + 3y' + 2y = 0
					</me>
				</p>
			</statement>

			<solution>
				<p>
					The characteristic equation is
				</p>

				<p>
					<md>
						<mrow>r^2 + 3r+2 \amp = 0 </mrow>
						<mrow> (r+2)(r+1) \amp = 0</mrow>
					</md>
				</p>

				<p>
					which has solutions <m>r=-2</m> and <m>r=-1</m>.
					The general solution thus is
				</p>

				<p>
					<me>
						y = c_1 e^{-2x} + c_2 e^{-x}
					</me>
				</p>
			</solution>
		</example>

		<p>
			To find the values of <m>c_1</m> and <m>c_2</m> in the example above or any other
			differential equation, additional information must be given.
			This is analogous to using a point to find the integration constant from an
			indefinite integral.
			The information is generally framed in the language of initial conditions and
			initial value problems as defined below.
		</p>

		<definition>
			<statement>
				<p>
					A differential equation has <term>initial conditions</term> if at some point
					<m>t_0</m>, then <m>y(t_0)</m>, <m>y'(t_0), \ldots, y^{(n-1)}(t_0)</m>
					are known, where <m>n</m> is the order of the differential equation.
					The differential equation together with the initial conditions is known as
					a <term>initial value problem</term>.
				</p>
			</statement>
		</definition>

		<p>
			The next example shows how to fully solve an initial value problem:
		</p>

		<example>
			<statement>
				<p>
					Find the solution to the initial value problem
				</p>

				<p>
					<me>
						y''+3y'+2y = 0 \qquad \text{$y(0)=3, y'(0) = -4$}.
					</me>
				</p>
			</statement>

			<solution>
				<p>
					To solve the initial value problem we first solve the differential equation,
					and this was done in <xref ref="ex-solution-DE-image" />
					And the general solution is
				</p>

				<p>
					<men xml:id="eq-ivp-ex1">
						y  = c_1 e^{-2x} + c_2 e^{-x}
					</men>
				</p>

				<p>
					Since the initial conditions include knowing the derivative, we will need
				</p>

				<p>
					<men xml:id="eq-ivp-ex2">
						y'  = -2c_1 e^{-2x} -c_2 e^{-x}
					</men>
				</p>

				<p>
					and then we will substitute <m>y(0)=3</m> into <xref ref="eq-ivp-ex1" />
					and <m>y'(0)=-4</m> into <xref ref="eq-ivp-ex2" />
				</p>

				<p>
					<md>
						<mrow>3 \amp = c_1 + c_2 </mrow>
						<mrow>-4 \amp = -2c_1 -c_2</mrow>
					</md>
				</p>

				<p>
					and the solution to this is <m>c_1=1</m> and <m>c_2=2</m>.
					Therefore the solution to the initial value problem is
				</p>

				<p>
					<me>
						y  = e^{-2x} + 2e^{-x}
					</me>
				</p>
			</solution>
		</example>

		<p>
			There are many general types of solutions to second-order constant coefficient differential equations.
			The following lemma shows the possible solutions.
		</p>

		<lemma xml:id="lem-soln-2nd-order-DE-homo">
			<statement>
				<p>
					Consider the general 2nd-order constant-coefficient linear homogeneous differential equation,
				</p>

				<p>
					<men xml:id="eq-general-2nd-order-DE-homo">
						a y'' + b y' + c y = 0
					</men>
				</p>

				<p>
					where <m>a, b</m> and <m>c</m> are real constants.
					Let <m>r_1</m>
					and <m>r_2</m> be the roots of the characteristic equation.
				</p>

				<p>
					<ol>
						<li>
							<p>
								If <m>r_1</m> and <m>r_2</m> are real and distinct, then the general solution to
								<xref ref="eq-general-2nd-order-DE-homo" /> is
							</p>

							<p>
								<men xml:id="eq-soln-2nd-order-DE-homo-eq1">
									y = c_1 e^{r_1 x} + c_2 e^{r_2 x}
								</men>
							</p>
						</li>

						<li>
							<p>
								If <m>r_1=r_2</m> is the only real root of the characteristic equation then the general
								solution to <xref ref="eq-general-2nd-order-DE-homo"/> is
							</p>

							<p>
								<men xml:id="eq-soln-2nd-order-DE-homo-eq2">
									y = e^{r_1 x} (c_1 + c_2 x )
								</men>
							</p>
						</li>

						<li>
							<p>
								If the roots of the characteristic equation are pure imaginary, that
								is <m>r_1=\beta i</m> and <m>r_2=-\beta i</m>, then the solution
								to <xref ref="eq-general-2nd-order-DE-homo"/> is
							</p>

							<p>
								<men xml:id="eq-soln-2nd-order-DE-homo-eq3">
									y = c_1 \sin \beta x + c_2 \cos \beta x
								</men>
							</p>
						</li>

						<li>
							<p>
								and if the roots of the characteristic equation are complex conjugates,
								that is <m>r_1=\alpha + \beta i </m> and <m>r_1=\alpha - \beta i </m>, then
								the solution to <xref ref="eq-general-2nd-order-DE-homo" /> is
							</p>

							<p>
								<men xml:id="eq-soln-2nd-order-DE-homo-eq4">
									y = e^{\alpha x} \bigl( c_1 \sin \beta x + c_2 \cos \beta x)
								</men>
							</p>
						</li>
					</ol>
				</p>
			</statement>


			<proof>
				<p>
					First, recall that the characteristic equation of <xref ref="eq-general-2nd-order-DE-homo" /> is
				</p>

				<p>
					<me>
						a r^2 + br+c = 0
					</me>
				</p>

				<p>
					We will prove each statement in order.
				</p>

				<p>
					<ol>
						<li>
							<p>
								The derivatives of <xref ref="eq-soln-2nd-order-DE-homo-eq1" /> are
							</p>

							<p>
								<md>
									<mrow>y' \amp = c_1 r_1 e^{r_1 x} + c_2 r_2 e^{r_2 x} </mrow>
									<mrow>y'' \amp = c_1 r_1^2 e^{r_1 x} + c_2 r_2^2 e^{r_2 x}</mrow>
								</md>
							</p>

							<p>
								and substituting these into <xref ref="eq-general-2nd-order-DE-homo" />,
							</p>

							<p>
								<md>
									<mrow>a y'' + b y' + c y \amp =
									a (c_1 r_1^2 e^{r_1 x} + c_2 r_2^2 e^{r_2 x}  ) + b(c_1 r_1 e^{r_1 x} </mrow>
									<mrow>\amp \qquad + c_2 r_2 e^{r_2 x}) + c(c_1 e^{r_1 x} + c_2 e^{r_2 x})</mrow>
								</md>
							</p>

							<p>
								rearranging
							</p>

							<p>
								<md>
									<mrow>\amp =  c_1 (a r_1^2 + b r_1 + c) e^{r_1 x} + c_2 (a r_2^2 + b r_2 + c) e^{r_2 x}</mrow>
								</md>
							</p>

							<p>
								and since <m>r_1</m> and <m>r_2</m> are roots of the characteristic equation,
								then both terms in parentheses are zero and
							</p>

							<p>
								<me>
									a y'' + b y' + c y =  0
								</me>
							</p>
						</li>

						<li>
							<p>
								The derivatives of <xref ref="eq-soln-2nd-order-DE-homo-eq2" /> are
							</p>

							<p>
								<md>
									<mrow>y' \amp = e^{r_1 x} (r_1 c_1 + c_2 + r_1 c_2  x ) </mrow>
									<mrow>y'' \amp = e^{r_1 x} (r_1^2 c_1 + 2 r_1 c_2 + r_1^2 c_2 x)</mrow>
								</md>
							</p>

							<p>
								where the product rule has been used.
								In this case, recall also that since <m>r_1</m> is the only real root,
								that <m>r_1 = -b/(2a)</m> from the quadratic formula with the discriminant <m>b^2-4ac=0</m>.
								Substituting into <xref ref="eq-general-2nd-order-DE-homo" />
							</p>

							<p>
								<md>
									<mrow>a y'' + by' + cy \amp = a e^{r_1 x} (r_1^2 c_1 + 2 r_1 c_2 + r_1^2 c_2 x) </mrow>
									<mrow>\amp  \qquad + be^{r_1 x} (r_1 c_1 + c_2 + r_1 c_2  x ) + c (c_1 + c_2 x )e^{r_1 x} </mrow>
									<mrow>\amp = \bigl( c_1 (a r_1^2 + b r_1 + c) + c_2 (2 a r_1 + b) </mrow>
									<mrow>\amp \qquad \qquad + c_2 x (a r_1^2  + br_1  + c)) \bigr) e^{r_1 x}  =0</mrow>
								</md>
							</p>

							<p>
								where the term with factor <m>c_1</m>  and the term with factor <m>c_2 x</m> are each 0,
								because <m>r_1</m> is a root of the characteristic equation.
								Lastly, the term with factor <m>c_2</m> is 0 because as stated about <m>r_1=-b/(2a)</m>.
							</p>
						</li>

						<li>
							<p>
								Note that since the roots are pure imaginary, then then <m>b=0</m> in
								<xref ref="eq-general-2nd-order-DE-homo" /> and therefore <m>r_1</m> and <m>r_2</m>
								satisfy <m>r^2=-c/a</m> and since <m>r_1=\beta i</m>, then <m>\beta^2=c/a</m>.
								The derivatives of <xref ref="eq-soln-2nd-order-DE-homo-eq3" /> are
							</p>

							<p>
								<md>
									<mrow>y' \amp = c_1 \beta \cos \beta x - c_2 \beta \sin \beta x </mrow>
									<mrow>y'' \amp = - c_1 \beta^2 \sin \beta x  -c_2 \beta^2 \cos \beta x</mrow>
								</md>
							</p>

							<p>
								and then substituting into <xref ref="eq-general-2nd-order-DE-homo" /> with <m>b=0</m>,
							</p>

							<p>
								<md>
									<mrow>ay'' + c y \amp = a (-c_1 \beta^2 \sin \beta x - c_2 \beta^2 \cos \beta x)
									+ c ( c_1 \sin \beta x  +c_2 \cos \beta x ) </mrow>
									<mrow>\amp = c_1 (-a\beta^2  + c) \sin \beta x + c_2 (-a\beta^2 +c) \cos \beta x =0
									</mrow>
								</md>
							</p>

							<p>
								since <m>\beta^2=c/a</m>.
							</p>
						</li>

						<li>
							<p>
								In this case, since the roots are complex conjugates,
								we can write <m>r_1=\alpha+i\beta </m> and <m>r_2=\alpha-i\beta</m>.
								The characteristic equation can be written:
							</p>

							<p>
								<md>
									<mrow>a(r-r_1)(r-r_2) \amp = a(r-(\alpha + i \beta))(r-(\alpha-i\beta)) </mrow>
									<mrow>\amp = a r^2 - 2 a \alpha r + a(\alpha^2+\beta^2) = 0</mrow>
								</md>
							</p>

							<p>
								which implies that <m>b=-2a \alpha</m> and <m>c=a(\alpha^2+\beta^2)</m>.
								The derivatives of <xref ref="eq-soln-2nd-order-DE-homo-eq4" /> are
							</p>

							<p>
								<md>
									<mrow>y' \amp = e^{\alpha x} \bigl( (c_1 \alpha - c_2 \beta) \sin \beta x + (c_2 \alpha + c_1 \beta) \cos \beta x \bigr) </mrow>
									<mrow>y'' \amp = e^{\alpha x} \bigl( (c_1 \alpha^2 -2 c_2 \alpha \beta - c_1 \beta^2) \sin \beta x </mrow>
									<mrow>\amp \qquad \qquad + (c_2 \alpha^2 + 2 c_1 \alpha \beta - c_2 \beta^2) \cos \beta x\bigr)</mrow>
								</md>
							</p>

							<p>
								and substituting them into <xref ref="eq-general-2nd-order-DE-homo" />,
							</p>

							<p>
								<md>
									<mrow>a y'' + by' + cy \amp = a e^{\alpha x} \bigl( (c_1 \alpha^2 -2 c_2 \alpha \beta - c_1 \beta^2) \sin \beta x </mrow>
									<mrow>\amp \qquad \qquad + (c_2 \alpha^2 + 2 c_1 \alpha \beta - c_2 \beta^2) \cos \beta x\bigr) </mrow>
									<mrow>\amp \qquad + b e^{\alpha x} \bigl( (c_1 \alpha - c_2 \beta) \sin \beta x + (c_2 \alpha + c_1 \beta) \cos \beta x \bigr)  </mrow>
									<mrow>\amp \qquad + c e^{ax} \bigl( c_1 \sin \beta x + c_2 \cos \beta x) </mrow>
									<mrow>\amp = e^{\alpha x} \bigl( c_1 (a\alpha^2-a\beta^2 +b\alpha + c) \sin \beta x </mrow>
									<mrow>\amp \qquad + c_1 (2a\alpha\beta+b\beta) \cos \beta x + c_2 (-2a\alpha \beta-b\beta) \sin \beta x  </mrow>
									<mrow number="yes" xml:id="eq-soln-2nd-order-DE-homo-eq4-proof">\amp \qquad + c_2 (a \alpha^2 - a \beta^2 + b \alpha + c) \bigr) </mrow>
								</md>
							</p>

							<p>
								And using <m>b=-2a\alpha</m> and <m>c=a(\alpha^2+\beta^2)</m>, the right hand side of
								<xref ref="eq-soln-2nd-order-DE-homo-eq4-proof" /> is 0, therefore
								<xref ref="eq-soln-2nd-order-DE-homo-eq4" /> is a solution.
							</p>
						</li>
					</ol>
				</p>
			</proof>
		</lemma>

		<example>
			<statement>
				<p>
					Find the general solution to  <m>y'' + 9y=0</m>.
				</p>
			</statement>

			<solution>
				<p>
					The characteristic equation is
				</p>

				<p>
					<md>
						<mrow>r^2+9 \amp = 0 </mrow>
						<mrow>r \amp = \pm 3i</mrow>
					</md>
				</p>

				<p>
					Since the roots are pure imaginary, the general solution is
				</p>

				<p>
					<md>
						<mrow>y \amp = C_1 \cos 3x + C_2 \sin 3x</mrow>
					</md>
				</p>
			</solution>
		</example>

		<p>
			The characteristic equation for this next example has complex roots.
		</p>

		<example>
			<statement>
				<p>
					Find the solution to <m>y'' + 4y' +5y=0</m>.
				</p>
			</statement>

			<solution>
				<p>
					The characteristic equation for this differential equation is
				</p>

				<p>
					<me>
						r^2 + 4r + 5  = 0
					</me>
				</p>

				<p>
					and since this can't be factored, we'll use the quadratic equation to solve this:
				</p>

				<p>
					<me>
						r = \frac{-4 \pm \sqrt{16-20}}{2} = -2 \pm i
					</me>
				</p>

				<p>
					Using <xref ref="lem-soln-2nd-order-DE-homo" />, the general solution is
				</p>

				<p>
					<md>
						<mrow>\amp = e^{-2x} \bigl( C_1 \cos x + C_2 \sin x \bigr)</mrow>
					</md>
				</p>

			</solution>
		</example>
	</subsection>

	<subsection>
		<title>Solutions Differential Equations as Vector Spaces</title>
		<p>
			We studied vector spaces in section <xref ref="sect-vector-spaces" /> and a common
			example of a vector space that is not <m>\mathbb{R}^n</m> is that of functions.
			It can be shown that the set related to the differential equation in
			<xref ref="ex-solution-DE-image" />
		</p>

		<p>
			<me>
				V  = \{ y \in \mathcal{C}^{(2)}(\mathbb{R}) \; | \; y'' + 9 y = 0 \}
			</me>
		</p>

		<p>
			is a vector space or a subspace of <m>\mathcal{C}^{(2)}</m>, the vector space of all functions with continuous 2nd derivatives.
			The basis of the subspace are the two solutions of the differential equation or <m>B=(\cos 3x, \sin 3x)</m>.
			Note that the general solution to the differential equation is the linear
			combination of the basis vectors or the span of the two solutions.
		</p>
	</subsection>
</section>