<?xml version="1.0" encoding="UTF-8"?>
<section xml:id="sect-linear-transformations">
	<title>Linear Transformations</title>
	<introduction>
		<p>
			This section
			discusses linear transformations.
			In short, such a
			transformation will map vectors to vectors in a linear way.
			The definition
			of a linear transformation (or linear map) is the following:
		</p>
		<definition
		xml:id="def-linear-trans">
		<title>Linear Transformation</title>
		<statement>
			<p>
				Let <m>V</m> and <m>W</m> be vector spaces.
				A <term>linear transformation</term> or <term>linear
				map</term> <m>T</m> from <m>V</m> to <m>W</m> is a function that assigns to each vector <m>\boldsymbol{v}
				\in V</m> a unique vector <m>T\boldsymbol{v} \in W</m> and that satisfies for each <m>\boldsymbol{u}</m>
				and <m>
				\boldsymbol{v}</m> in <m>V</m> and each scalar <m>\alpha</m>,
				<md>
					<mrow xml:id="eq-linear-map-add" number="yes">(\boldsymbol{u} + \boldsymbol{v}) \amp = T(\boldsymbol{u}) + T
					(\boldsymbol{v}), </mrow>
					<mrow xml:id="eq-linear-map-prod" number="yes">T(\alpha \boldsymbol{v}) \amp = \alpha T
					(\boldsymbol{v}), </mrow>
				</md>
			</p>
		</statement>
	</definition>

	<p>
		These are also called <term>
		homomorphisms</term> and the notation explaining that a map <m>T</m> goes from <m>V</m> to <m>
		W</m> is <m>T: V \rightarrow W</m>.
	</p>

	<example xml:id="ex-reflect-map">
		<title>Reflection Map</title>
		<statement>
			<p>
				The reflection of any vector in <m>\mathbb{R}^2</m> across the horizontal axis is a
				linear map.
				Specifically this is given as
			</p>

			<p>
				<me>
					T(\begin{bmatrix}
					x_1 \\ x_2
					\end{bmatrix})= \begin{bmatrix}
					x_1 \\ -x_2
					\end{bmatrix}
				</me>
			</p>

			<p>
				and geometrically you can see this as:
			</p>

			<figure xml:id="fig-reflection-map">
				<caption>Mapping a vector over the <m>x</m>-axis</caption>
				<image width="50%" xml:id="plot-reflection-map">
					<latex-image>
					<![CDATA[
					\begin{tikzpicture}[scale=1.5]
					\draw[->] (-1,0) -- (2,0);  \draw[->] (0,-1) -- (0,1);
					\draw[->, thick] (0,0) -- (1.5,0.5) node [above right] {$\displaystyle \begin{bmatrix}
					x_1 \\ x_2
					\end{bmatrix}$};
					\draw[->, thick] (0,0) -- (1.5,-0.5) node [below right] {$\displaystyle \begin{bmatrix}
					x_1 \\ -x_2
					\end{bmatrix}$};
					\end{tikzpicture}
					]]>
					</latex-image>
				</image>
			</figure>

			<p>
				Show that this is a linear transformation.
			</p>
		</statement>

		<solution>
			<p>
				Specifically, we need to show that <m>T</m> defined above satisfies <xref
				ref="eq-linear-map-add" /> and <xref ref="eq-linear-map-prod" />.
				Let
			</p>

			<p>
				<md>
					<mrow>\boldsymbol{x} \amp = \begin{bmatrix}
					x_1 \\ x_2
					\end{bmatrix}, \amp \boldsymbol{y} \amp = \begin{bmatrix}
					y_1 \\ y_2
					\end{bmatrix}
					</mrow>
				</md>
			</p>

			<p>
				and
			</p>

			<p>
				<m>\alpha \in \mathbb{R}</m>, then
			</p>

			<p>
				<md>
					<mrow>T(\boldsymbol{x}+\boldsymbol{y}) \amp = T \biggl( \begin{bmatrix}
					x_1 \\ x_2
					\end{bmatrix}+ \begin{bmatrix}
					y_1 \\ y_2
					\end{bmatrix} \biggr) = T \biggl( \begin{bmatrix}
					x_1 + y_1 \\ x_2 + y_2
					\end{bmatrix} \biggr) </mrow>
					<mrow>\amp = \begin{bmatrix}
					x_1 + y_1 \\ -(x_2+y_2)
					\end{bmatrix} = \begin{bmatrix}
					x_1 + y_1 \\ -x_2 -y_2
					\end{bmatrix} </mrow>
					<mrow>\amp = \begin{bmatrix}
					x_1 \\ -x_2
					\end{bmatrix} + \begin{bmatrix}
					y_1 \\ -y_2
					\end{bmatrix} = T(\boldsymbol{x}) + T(\boldsymbol{y}).</mrow>
				</md>
			</p>

			<p>
				so <xref ref="eq-linear-map-add" /> is satisfied.
				Next,
			</p>

			<p>
				<md>
					<mrow>T(\alpha \boldsymbol{x}) \amp = T \biggl( \alpha \begin{bmatrix}
					x_1 \\ x_2
					\end{bmatrix} \biggr) = T \biggl( \begin{bmatrix}
					\alpha x_1 \\ \alpha x_2
					\end{bmatrix} \biggr) </mrow>
					<mrow>\amp = \begin{bmatrix}
					\alpha x_1 \\ -\alpha x_2
					\end{bmatrix} = \alpha \begin{bmatrix}
					x_1 \\ -x_2
					\end{bmatrix} = \alpha T(\boldsymbol{x}).</mrow>
				</md>
			</p>

			<p>
				so <xref
				ref="eq-linear-map-prod" /> is satisfied.
			</p>
		</solution>
	</example>

	<p>
		A very important linear map in <m>\mathbb{R}^2</m> is the rotational map that takes any
		vector in the plane and rotates it a given angle.
		The next example, derives this map.
	</p>

	<example xml:id="ex-rotational-trans">
		<title>Rotational Map in <m>\mathbb{R}^2</m></title>
		<statement>
			<p>
				Let
				<me>
					\boldsymbol{x} =
					\begin{bmatrix}
					x_1 \\ x_2
					\end{bmatrix}
				</me>
				be a vector in <m>\mathbb{R}^2</m>.
				Let the function <m>T</m> take
				the vector <m>\boldsymbol{x}</m> and rotate it by <m>\theta</m> radians in the counterclockwise
				direction.
				Call the new vector
				<me>
					\boldsymbol{y} =\begin{bmatrix}
					y_1 \\ y_2
					\end{bmatrix}
				</me>
			</p>

			<figure xml:id="fig-rotational-map">
				<caption>Diagram of the rotational map</caption>
				<image width="50%" xml:id="plot-rotational-map">
					<latex-image>
					<![CDATA[
					\begin{tikzpicture}[scale=1.5]
					\draw (0.2,0.2) node [above right] {$ \theta $};
					\draw[->] (-2,0) -- (2,0);  \draw[->] (0,-2) -- (0,2);
					\draw[->, thick] (0,0) -- (1.5,0.5);   \fill (1.5,0.5) circle (1pt) node [above right] {$ (x_1,x_2) $};
					\draw[->,thick] (0,0) -- (0.5,1.5); \fill (0.5,1.5) circle (1pt) node [above right] {$ (y_1,y_2) $};
					\draw (0.3,0.1) arc [start angle={atan(1/3)}, end angle={atan(3)}, radius={sqrt(0.1)}];
					\draw (0.45,0) arc [start angle=0, end angle={atan(1/3)}, radius=0.45];
					\draw (0.6,0) node [above right] {$ \alpha $};
					\end{tikzpicture}
					]]>
					</latex-image>
				</image>
			</figure>

			<p>
				Derive the formula for the rotational map.
			</p>
		</statement>

		<solution>
			<p>
				Let <m>r = ||\boldsymbol{x}||</m> and since <m>\boldsymbol{y}</m> is the rotated version of <m>\boldsymbol{x}</m>
				it has the same length, therefore <m>r=||\boldsymbol{y}||</m>.
				The values <m>x_1, x_2, y_1,y_2</m>
				can be written in terms of <m>\alpha</m>, the angle that the vector <m>\boldsymbol{x}</m> makes
				with the positive horizontal axis, and <m>\theta</m> the angle between the vectors as
				follows.
			</p>

			<p>
				<md>
					<mrow>x_1 \amp = r \cos \alpha, \amp x_2 \amp = r \sin \alpha, </mrow>
					<mrow>y_1 \amp = r \cos (\alpha+\theta), \amp y_2 \amp= r \sin (\alpha + \theta) </mrow>
					<mrow>\amp = r \cos \alpha \cos \theta - r \sin \theta \sin \alpha, \amp y_2 \amp = r
					\sin
					\theta \cos \alpha + r \sin \alpha \cos \theta </mrow>
					<mrow>\amp = x_1 \cos \theta - x_2 \sin \theta, \amp \amp = x_1 \sin \theta + x_2 \cos
					\theta</mrow>
				</md>
			</p>

			<p>
				and note that these can be written:
			</p>

			<p>
				<md>
					<mrow>\begin{bmatrix}
					y_1 \\ y_2
					\end{bmatrix} \amp =
					\begin{bmatrix}
					\cos \theta \amp - \sin \theta \\ \sin \theta \amp \cos \theta
					\end{bmatrix}
					\begin{bmatrix}
					x_1 \\ x_2
					\end{bmatrix}
					</mrow>
				</md>
			</p>

			<p>
				This is a linear transformation (as we will explain later) and is called a <term>rotational
				transformation</term>.
			</p>
		</solution>
	</example>

	<example xml:id="ex-scale-map">
		<title>Linear Scale Map</title>
		<statement>
			<p>
				Consider the map <m>S: \mathbb{R}^2 \rightarrow \mathbb{R}^2</m> that scales any vector
				in the plane by a factor of <m>k</m> given by
			</p>

			<p>
				<me>
					S(\boldsymbol{x}) = k \boldsymbol{x}
				</me>
			</p>

			<p>
				which can be visualized in the following diagram where <m> k=2</m>:
			</p>

			<figure xml:id="fig-scale-map">
				<caption>Scaling Map</caption>
				<image width="50%" xml:id="plot-scale-map">
					<latex-image>
					<![CDATA[
					\begin{tikzpicture}[scale=0.8]
					\draw[->] (-4,0) -- (4,0) node [above right] {$ x $};
					\draw[->] (0,-4) -- (0,4) node [above right] {$ y $};
					\foreach \x in {-3,-2,-1,1,2,3} {\draw (\x,0.15) -- (\x,-0.15) node [below] {$ \x $};}
					\foreach \y in {-3,-2,-1,1,2,3} {\draw (0.15,\y) -- (-0.15,\y) node [left] {$ \y $};}
					\draw[->,decoration={markings,mark=at position 0.9999 with {\arrow[scale=4,blue]{>}}}] (0,0) -- (1,1); \draw[->,thick] (0,0)  -- (2,2);
					\draw[->] (0,0) -- (2,1); \draw[->,thick] (0,0)  -- (4,2);
					\draw[->] (0,0) -- (-1,1.5); \draw[->,thick] (0,0)  -- (-2,3);
					\draw[->] (0,0) -- (-1.5,-1); \draw[->,thick] (0,0)  -- (-3,-2);
					\end{tikzpicture}
					]]>
					</latex-image>
				</image>
			</figure>

			<p>
				where every vector under the map results in a new vector that is twice as long as the
				original.
				In general, the scale <m>k</m> will scale the vector by a factor of <m>k</m> and
				recall that if <m>k \lt 0</m>, then the direction changes.
				Show that this is a linear map.
			</p>
		</statement>

		<solution>
			<p>
				Again, we show that <xref ref="eq-linear-map-add" /> and <xref
				ref="eq-linear-map-prod" /> are satisfied.
				Let <m>\boldsymbol{x}</m> and <m>\boldsymbol{y}</m> be
				elements of <m>\mathbb{R}^2</m>.
			</p>

			<p>
				<me>
					S(\boldsymbol{x}+\boldsymbol{y}) = k(\boldsymbol{x}+\boldsymbol{y}) = k\boldsymbol{x} + k \boldsymbol{y} = S(\boldsymbol{x}) + S(\boldsymbol{y})
				</me>
			</p>

			<p>
				so <xref ref="eq-linear-map-add" /> is satisfied and
			</p>

			<p>
				<me>
					S(\alpha \boldsymbol{x}) = k (\alpha \boldsymbol{x} ) = \alpha (k \boldsymbol{x}) = \alpha S(\boldsymbol{x})
				</me>
			</p>

			<p>
				so <xref ref="eq-linear-map-add" /> is satisfied so <m>S</m> is a linear map.
			</p>
		</solution>
	</example>
	<theorem
	xml:id="thm-matrix-linear-trans">
	<statement>
		<p>
			If a transformation map <m>T</m> is written as a matrix or <m>T(\boldsymbol{x}) = A\boldsymbol{x}</m>,
			then <m>T</m> is a linear transformation.
		</p>
	</statement>


	<proof>
		<p>
			This is a consequence of matrix operations.
			<md>
				<mrow>T(\boldsymbol{x}+\boldsymbol{y}) &amp;= A(\boldsymbol{x}+\boldsymbol{y}) = A\boldsymbol{x} + A \boldsymbol{y} = T(\boldsymbol{x}) +
				T(\boldsymbol{y}) </mrow>
				<mrow>T(\alpha \boldsymbol{x}) &amp; = A (\alpha \boldsymbol{x}) = \alpha A\boldsymbol{x} = \alpha T(\boldsymbol{x}).</mrow>
			</md>
		</p>
	</proof>
</theorem>

<p>
	Note that the rotational transformation that was defined in  <xref ref="ex-rotational-trans" /> is easily
	shown to be a linear transformation because from  <xref ref="thm-matrix-linear-trans" />, any
	transformation shown as a matrix, is a linear transformation.
	The next theorem shows the counter direction to <xref ref="thm-matrix-linear-trans" />,
	that is that any linear transformation can be written as a matrix.
</p>

<theorem xml:id="thm-linear-trans-matrix">
	<statement>
		<p>
			Let <m>T: \mathbb{R}^n \rightarrow \mathbb{R}^m</m> be a linear transformation.
			Then
			there exists a unique <m>m</m> by <m>n</m> matrix <m>A_T</m> such that
			<me>
				T \boldsymbol{x} = A_T \boldsymbol{x} \qquad \qquad \text{for every $\boldsymbol{x} \in \mathbb{R}^n.$}
			</me>
		</p>
	</statement>
</theorem>

<p>
	We won't prove this here, but instead will motivate this below.
	In short, if <m>
	T</m> is a linear transformation, then the matrix <m>A_T</m> corresponding to the linear
	transformation is called the <term>transformation matrix</term>.
</p>
</introduction>

<subsection>
	<title>Finding the
	Matrix Form of a Linear Transformation</title>
	<p>
		The theorem above shows that any linear
		transformation, <m>T: V \rightarrow W</m> can be written in matrix form.
		This section explains
		how to find it.
		Let <m>B_V=(\boldsymbol{v}_1,\boldsymbol{v}_2, \ldots, \boldsymbol{v}_m)</m> be a basis of <m>V</m>
		and <m>B_W=(\boldsymbol{w}_1,\boldsymbol{w}_2,
		\ldots, \boldsymbol{w}_n)</m> be a basis of <m>W</m>.
		Any vector <m>\boldsymbol{x}</m> in <m>V</m> can be
		written
		<me>
			\boldsymbol{x} = c_1 \boldsymbol{v}_1 + c_2 \boldsymbol{v}_2 + \cdots + c_m \boldsymbol{v}_m = \sum_{j=1}^m c_j
			\boldsymbol{v}_j
		</me>
		or in other words <m>\text{Rep}_{B_V}(\boldsymbol{x}) = \boldsymbol{c}</m>.
		Applying the map to <m>\boldsymbol{x}</m>
		is
		<me>
			T(\boldsymbol{x}) = T\biggl(\sum_{j=1}^m c_j \boldsymbol{v}_j \biggr) \notag
		</me>
		and since it is a linear map
		<men xml:id="eq-lin-trans1">
			T(\boldsymbol{x})= \sum_{j=1}^m c_j T(\boldsymbol{v}_j)
		</men>
		Next, we write the transformation in terms of the basis vectors of <m>W</m> or
		<men xml:id="eq-lin-trans2">
			T(\boldsymbol{v}_j) = a_{1,j} \boldsymbol{w}_1 + a_{2,j} \boldsymbol{w}_2 + \cdots + a_{n,j} \boldsymbol{w}_n =
			\sum_{i=1}^n a_{i,j} \boldsymbol{w}_i
		</men>
		Substituting <xref ref="eq-lin-trans2" /> into <xref ref="eq-lin-trans1" /> results in
		<me>
			T(\boldsymbol{x}) = \sum_{j=1}^m c_j \sum_{i=1}^n a_{i,j} \boldsymbol{w}_i
			= \sum_{i=1}^n \sum_{j=1}^m a_{i,j} c_j \boldsymbol{w}_i
		</me>
		and letting <m>A_T</m> be the <m>m \times n</m> matrix with entries <m>a_{i,j}</m> then
		<me>
			\text{Rep}_{B_W} (T(\boldsymbol{x}))  = A_T\boldsymbol{c}
		</me>
		or in other words, the matrix
		performs the map on the coefficients.
		Equation <xref ref="eq-lin-trans2" /> also shows how the
		matrix <m>A_T</m> can be created from the linear map.
		That equation can also be thought of as a
		representation of the basis vectors or
		<me>
			\text{Rep}_{B_W} ( T(\boldsymbol{v}_j)) = \boldsymbol{a}_j
		</me>
		where <m>a_j</m> is the <m>j</m>th
		column of <m>A</m>.
		The following summarizes how to find the matrix.
	</p>

	<remark>
		<p>
			If <m>A_T</m> is
			the matrix representation of the map <m>T</m>, then the <m>j</m>th column of <m>A_T</m> is the
			vector <m>
			\text{Rep}_{B_W}(T(\boldsymbol{v}_j))</m>, the map applied to the <m>j</m>th basis vector of <m>V</m>
			written in terms of the basis of <m>W</m>.
		</p>
	</remark>

	<p>
		We now show many examples on how to apply
		this.
	</p>

	<example>
		<statement>
			<p>
				The matrix representation of the reflection map from <xref ref="ex-reflect-map" /> given by
			</p>

			<p>
				<me>
					T\biggl(\begin{bmatrix}
					x_1 \\ x_2
					\end{bmatrix} \biggr) = \begin{bmatrix}
					x_1 \\ -x_2
					\end{bmatrix}
				</me>
			</p>

			<p>
				where the representation will be in terms of the standard basis vectors.
			</p>
		</statement>

		<solution>
			<p>
				In this case,
				we need to determine how the standard basis vectors map under the reflection.
				Thus
			</p>

			<p>
				<md>
					<mrow>   \boldsymbol{v}_1 \amp = \begin{bmatrix}
					1 \\ 0
					\end{bmatrix} \amp \boldsymbol{v}_2 = \begin{bmatrix}
					0 \\ 1
					\end{bmatrix}</mrow>
				</md>
			</p>

			<p>
				and
			</p>

			<p>
				<md>
					<mrow>T(\boldsymbol{v}_1) \amp = \begin{bmatrix}
					1 \\ 0
					\end{bmatrix} \amp T(\boldsymbol{v}_2) \amp = \begin{bmatrix}
					0 \\ -1
					\end{bmatrix}</mrow>
				</md>
			</p>

			<p>
				Because we are using the standard basis vectors, the representations of these vectors are
				themselves therefore,
			</p>

			<p>
				<me>
					A_T = \begin{bmatrix}
					1 \amp 0 \\
					0 \amp -1
					\end{bmatrix}
				</me>
			</p>

			<p>
				and just to verify,
			</p>

			<p>
				<md>
					<mrow>T\biggl(\begin{bmatrix}
					x_1 \\ x_2
					\end{bmatrix} \biggr) \amp = \begin{bmatrix}
					1 \amp 0 \\
					0 \amp -1
					\end{bmatrix} \begin{bmatrix}
					x_1 \\ x_2
					\end{bmatrix} = \begin{bmatrix}
					x_1 \\ - x_2
					\end{bmatrix}</mrow>
				</md>
			</p>
		</solution>
	</example>

	<p>
		This next example shows how to contruct the transformation matrix for
		the scale map.
	</p>

	<example xml:id="ex-scale-map-matrix-rep">
		<statement>
			<p>
				Find the matrix representation of the scale map in <xref ref="ex-scale-map" />.
			</p>
		</statement>
		<solution>
			<p>
			We need to map the basis vectors <m>[1\;\;0]^{\intercal}</m> and
			<m>[0\;\;1]^{\intercal}</m> to determine the columns of the matrix representation.
			</p>

			<p>
				<md>
					<mrow>
					S \biggl(\begin{bmatrix}
					1 \\ 0
					\end{bmatrix} \biggr) \amp = \begin{bmatrix}
					k \\ 0
					\end{bmatrix} \amp S\biggl( \begin{bmatrix}
					0 \\ 1
					\end{bmatrix} \biggr) \amp = \begin{bmatrix}
					0 \\ k
					\end{bmatrix}</mrow>
				</md>
			</p>

			<p>
				so the matrix representation is
			</p>

			<p>
				<me>
					A_S = \begin{bmatrix}
					k \amp 0 \\
					0 \amp k
					\end{bmatrix}
				</me>
			</p>
		</solution>
	</example>

	<p>
		And the next example shows that a common matrix operation, the trace
		is a linear map.
	</p>

	<example>
		<statement>
			<p>
				Let <m>T: \mathcal{M}_{2 \times 2} \rightarrow \mathbb{R}</m>
			</p>

			<p>
				<me>
					\begin{bmatrix}
					a \amp b \\ c\amp d
					\end{bmatrix} \rightarrow a + d
				</me>
			</p>

			<p>
				which is the trace of a 2 by 2 matrix.
				Show that the trace is a linear map and find the matrix
				representation of the trace.
			</p>
		</statement>

		<solution>
			<p>
				First, to prove that the trace is a linear map, we need
				to show that it satisfies <xref ref="eq-linear-map-add" /> and <xref ref="eq-linear-map-prod" />.
				Let
			</p>

			<p>
				<md>
					<mrow>A_1 \amp = \begin{bmatrix}
					a_1 \amp b_1 \\ c_1\amp d_1
					\end{bmatrix} \amp A_2 \amp = \begin{bmatrix}
					a_2 \amp b_2 \\ c_2\amp d_2
					\end{bmatrix}
					</mrow>
				</md>
			</p>

			<p>
				Then
			</p>

			<p>
				<md>
					<mrow>T(A_1+A_2) \amp = T \left( \begin{bmatrix}
					a_1 \amp b_1 \\ c_1\amp d_1
					\end{bmatrix} + \begin{bmatrix}
					a_2 \amp b_2 \\ c_2\amp d_2
					\end{bmatrix} \right) = T \left( \begin{bmatrix}
					a_1 + a_2 \amp b_1 + b_2 \\ c_1 + c_2 \amp d_1 + d_2
					\end{bmatrix} \right) </mrow>
					<mrow>\amp = (a_1 + a_2) + (d_1 + d_2) \\
					\amp = (a_1 + d_1) + (a_2 + d_2) = T(A_1) + T(A_2)
					</mrow>
				</md>
			</p>

			<p>
				Similarly,
			</p>

			<p>
				<md>
					<mrow>T(\alpha A_1) \amp = T \biggl( \alpha \begin{bmatrix}
					a_1 \amp b_1 \\ c_1\amp d_1
					\end{bmatrix}\biggr) = T\biggl(\begin{bmatrix}
					\alpha a_1 \amp \alpha b_1 \\ \alpha c_1\amp \alpha d_1
					\end{bmatrix} \biggr) </mrow>
					<mrow>\amp = \alpha a_1 + \alpha d_1 = \alpha (a_1 + d_1) = \alpha T(A_1)
					</mrow>
				</md>
			</p>

			<p>
				Next, we want to find the matrix representation of the trace.
				To do this, we need to determine
				how the map affects the basis of the vector space <m>\mathcal{M}_{2 \times 2}</m>, which is
			</p>

			<p>
				<me>
					\left( \begin{bmatrix}
					1 \amp 0 \\ 0 \amp 0
					\end{bmatrix}, \begin{bmatrix}
					0 \amp 1 \\ 0 \amp 0
					\end{bmatrix}, \begin{bmatrix}
					0 \amp 0 \\ 1 \amp 0
					\end{bmatrix}, \begin{bmatrix}
					0 \amp 0 \\ 0 \amp 1
					\end{bmatrix} \right)
				</me>
			</p>

			<p>
				and since
			</p>

			<p>
				<md>
					<mrow>\begin{bmatrix}
					1 \amp 0 \\ 0 \amp 0
					\end{bmatrix} \amp\mapsto 1, \amp
					\begin{bmatrix}
					0 \amp 1 \\ 0 \amp 0
					\end{bmatrix} \amp\mapsto 0, </mrow>
					<mrow>
					\begin{bmatrix}
					0 \amp 0 \\ 1 \amp 0
					\end{bmatrix} \amp\mapsto 0, \amp
					\begin{bmatrix}
					0 \amp 0 \\ 0 \amp 1
					\end{bmatrix} \amp \mapsto 1, </mrow>
				</md>
				The matrix representation is
				<me>
					A_T = \begin{bmatrix}
					1 \amp 0 \amp 0 \amp 1
					\end{bmatrix}
				</me>
				Note that it may be surprising that the matrix representation is just a row
				vector, however, recall that the trace maps from a <m>2 \times 2</m> matrix
				that can be represented as a column vector of length 4 to the reals, so the
				matrix representation should be a <m>1 \times 4</m> matrix.
			</p>
		</solution>
	</example>

	<p>
		To verify the above results, recall that from <xref ref="ex-vect-rep-matrix" /> that the
		representation of a matrix is the unfolded matrix or in the <m>2 \times 2</m> case, that
		<me>
			\text{Rep}_B \biggl( \begin{bmatrix}
			a \amp b \\ c \amp d
			\end{bmatrix}\biggr) = \begin{bmatrix}
			a \\ b \\ c \\ d
			\end{bmatrix}
		</me>
		where <m>B</m> is the natural basis of <m>\mathcal{M}_{2 \times 2}</m>.
		So the matrix trace can
		be written as
		<me>
			\begin{bmatrix}
			1 \amp 0 \amp 0 \amp 1
			\end{bmatrix}\text{Rep}_B (A) = \begin{bmatrix}
			1 \amp 0 \amp 0 \amp 1
			\end{bmatrix}\begin{bmatrix}
			a \\ b \\ c \\ d
			\end{bmatrix} = a + d
		</me>
	</p>
</subsection>
</section>